nola/examples/mutex.v
@@ -5,9 +5,9 @@ From nola.rust_lang Require Export notation proofmode.
 Import FunPRNotation ModwNotation WpwNotation DsemNotation LftNotation.
 
 Section mutex_bor.
-  Context `{!lrustGS_gen hlc Σ, !SemCifcon JUDG CON Σ, !Jsem JUDG (iProp Σ),
-    !inv'GS (cifOF CON) Σ, !InvCon CON, !InvSem JUDG CON Σ,
-    !borrowGS (cifOF CON) Σ, !BorCon CON, !BorSem JUDG CON Σ}.
+  Context `{!lrustGS_gen hlc Σ, !SemCifcon CON JUDG Σ, !Jsem JUDG (iProp Σ),
+    !inv'GS (cifOF CON) Σ, !InvCon CON, !InvSem CON JUDG Σ,
+    !borrowGS (cifOF CON) Σ, !BorCon CON, !BorSem CON JUDG Σ}.
   Implicit Type (Px Qx : cif CON Σ) (Φx Ψx : loc → cif CON Σ) (b : bool)
     (l : loc).
 
